---
title: "Sekhar_Mekala_HW2"
author: "Sekhar Mekala"
date: "Monday, September 12, 2016"
output: pdf_document
---

![Question_1](C:\Users\Sekhar\Documents\R Programs\Simulation\HW2\Q1.png)
*Answer:*

Given the following probability mass function (pmf):

$$Pr(X=k) = ck^2, \mbox{ where } k=1,2,3$$  

Therefore the sum of probabilities on all the values of $k=1,2,3$ will be 1.

$$\sum_{k=1}^{3} ck^2 = 1$$
$$c(1) +c(2^2)+c(3^2) = 1$$
$$c = \frac{1}{14}$$

Therefore, the $pmf$ can be written as:

$$Pr(X=k) = \frac{k^2}{14}, \mbox{ where } k=1,2,3$$  

*Let us find the $Pr(X \leq 2)$*

$$Pr(x \leq 2) = Pr(x=1) + Pr(x=2) = \frac{1}{14} + \frac{4}{14} = \frac{5}{14}$$

*Let us find the E[X]*

$$E[X] = \sum_{k=1}^{3} k.k^2/14 = \sum_{k=1}^{3} k^3/14 = \frac{1^3+2^3+3^3}{14} = \frac{36}{14} = \frac{18}{7}$$

*Deriving V[X]*

$$V[X] = E[X^2] - (E[X])^2$$

$$E[X^2] = \sum_{k=1}^{3} k^2.k^2/14 = \sum_{k=1}^{3} k^4/14 = \frac{1^4 + 2^4 + 3^4}{14} = \frac{1+16+81}{14} = 7$$
We already know that $E[X] = \frac{18}{7}$

Therefore,
$$V[X] = E[X^2] - (E[X])^2 = 7 - (\frac{18}{7})^2 = 0.38775$$


![Question_2](C:\Users\Sekhar\Documents\R Programs\Simulation\HW2\Q2.png)
*Answer:*

Given that $p.d.f$ as 
$$f(x) = cx^2 \mbox{ where } x \in [1,2]$$

*Finding the value of c*

$${\displaystyle \int_{1}^{2} cx^2 \mbox{ } dx = 1}$$
$${\displaystyle \frac{c.2^3}{3} - \frac{c.1^3}{3} = 1}$$
$$c = \frac{3}{7}$$

*Finding $pr(X \geq 1)$*

$$pr(x \geq 1) = \int_{1}^{\infty} (3/7)x^2 \mbox{ } dx$$

But $x \in [1,2]$, hence

$$pr(x \geq 1) = \int_{1}^{2} (3/7)x^2 \mbox{ } dx = \frac{2^3}{7} - \frac{1^3}{7} = 1$$

*Finding E[X]*

$${\displaystyle E[X] = \int_{1}^{2} (3/7)x^2 . x \mbox{ } dx = \left[(3/7) (x^4/4)\right]_1^2 = \left[3x^4/28 \right]_{1}^{2} = \frac{45}{28}}$$

*Finding V[X]*

$$V[X] = E[X^2] - (E[X])^2$$

$$E[X^2] = \int_{1}^{2} (3/7)x^2 . x^2 \mbox{ } dx = \int_{1}^{2} (3/7)x^4 \mbox{ } dx = \left[ (3/35)x^5 \right]_1^2 = \frac{93}{35}$$

We know that $E[X] = \frac{45}{28}$

Therefore,

$$V[X] = E[X^2] - (E[X])^2 = \frac{93}{35} - (\frac{45}{28})^2 = 2.657-2.583 = 0.074$$

![Question_3](C:\Users\Sekhar\Documents\R Programs\Simulation\HW2\Q3.png)
*Answer:*

*Finding $f_x(x)$*

$$\int_{1}^{2} (y-x) dy = \left[ \frac{y^2}{2} - xy \right]_1^2 = \frac{3}{2} - x$$


*Finding $f_y(y)$*

$$\int_{0}^{1} (y-x) dx = \left[ yx - \frac{x^2}{2} \right]_0^1 = y - \frac{1}{2}$$

*Drawing $f_x(x)$ in the interval x=[0,1]*

```{r echo=FALSE}
library(ggplot2)


draw_fun_x <- function(x)
{

return((3/2) - x)

}


ggplot(data.frame((x=c(0,1))),aes(x))+
  stat_function(fun=draw_fun_x,color="red")+
  labs(title="f(x) = 3/2 - x",y="f(x)")

```

*Drawing $f_y(y) in the interval y=[1,2]$*

```{r echo=FALSE}
draw_fun_y <- function(y)
{

return(y - (1/2))

}

library(ggplot2)


ggplot(data.frame((x=c(1,2))),aes(x))+
  stat_function(fun=draw_fun_y,color="red")+
  labs(title="f(y) = y - (1/2)",y="f(y)",x="y")

```

*Checking if X and Y are independent*

X and Y are independent, if $f(X,Y) = f_x(x) f_y(y)$

Given that $f(x,y) = y-x$ and $f_x(x) f_y(y) = ((3/2)-x)(y-(1/2)) = (3/2)y - xy - (3/4) +(x/2)$

Since $f(X,Y) \neq f_x(x) f_y(y)$, x and y are not independent.


##Computing $F_x(x)$

$$F_x(x) = \int_0^x f_x(x) dx$$
$$F_x(x) = \int_0^x ((3/2) - t) dt = \left[1.5t - (t^2/2)\right]_0^x = 1.5x - \frac{x^2}{2}$$
Therefore, 
$$F_x(x) = 1.5x - \frac{x^2}{2}\mbox{ when } x \in [0,1]$$
$$F_x(x) = 0 \mbox{ when } x \leq 0$$
$$F_x(x) = 1 \mbox{ when } x \geq 1$$

##Computing $F_y(y)$

$$F_y(y) = \int_1^y f_y(y) dy$$
$$F_y(y) = \int_1^y (t - (1/2)) dt = \left[t^2/2 - (1/2)t\right]_1^y = 0.5y^2 - 0.5y$$
Therefore, 
$$F_y(y) = 0.5y^2 - 0.5y\mbox{ when } y \in [1,2]$$
$$F_y(y) = 0 \mbox{ when } y \leq 1$$
$$F_y(y) = 1 \mbox{ when } y \geq 2$$


##Computing $E[X]$

$$E[X] = \int_0^1 x.f_X(x) \mbox{ } dx = \int_0^1 (3/2)x-x^2 \mbox{ } dx = \left[(3/4)x^2 - (x^3/3) \right]_{0}^{1} = (3/4)-(1/3) = 5/12 = 0.417$$

##Computing $V[X]$

$$V[X] = E[X^2] - (E[X])^2$$

$$E[X^2] = \int_0^1 x^2.f_X(x) \mbox{ } dx = \int_0^1 (3/2)x^2-x^3 \mbox{ } dx = \left[(1/2)x^3 - (x^4/4) \right]_{0}^{1} = (1/2)-(1/4) = 1/4 = 0.25$$

$$V[X] = E[X^2] - (E[X])^2 = 0.25 - (5/12)^2 = 0.07638889$$

##Computing $E[Y]$

$$E[Y] = \int_1^2 y.f_Y(y) \mbox{ } dy = \int_1^2 y^2-(y/2) \mbox{ } dy $$ 
$$E[Y] = \left[(y^3/3) - (y^2/4) \right]_{1}^{2} = (8/3)-(4/4) - (1/3) + (1/4) = (7/3) - (3/4) = 19/12 = 1.583333$$

##Computing $V[Y]$

$$V[Y] = E[Y^2] - (E[Y])^2$$

$$E[Y^2] = \int_1^2 y^2.f_Y(y) \mbox{ } dy = \int_1^2 y^3 - (1/2)y^2 \mbox{ } dy = \left[y^4/4 - (y^3/6) \right]_{1}^{2} = 31/12$$

$$V[Y] = E[y^2] - (E[y])^2 = 31/12 - (19/12)^2 = 0.07638889$$


##Computing $Cov(X,Y)$

$$Cov(X,Y) = E[XY] - E[X].E[Y]$$

$$E[XY] = \int_0^1 \int_1^2 (x.y.(y - x) \mbox{ }dy) \mbox{ }dx $$
$$E[XY] = \int_0^1 \int_1^2 (x.y^2 - x^2.y) \mbox{ }dy) \mbox{ }dx$$
$$E[XY] = \int_0^1 \left[(x.y^3/3) - (x^2.y^2/2) \right]_1^2 \ \mbox{ }dx = \int_0^1 (7x/3) - (3x^2/2) \mbox{ }dx$$
$$E[XY] = \left [ (7x^2/6 - (3x^3/6) \right]_0^1 = 2/3$$

$$Cov(X,Y) = E[XY] - E[X].E[Y] = (2/3) - (5/12)(19/12) = 0.006944444$$

##Computing $Corr(X,Y)$

$$Corr(X,Y) = \frac{Cov(X,Y)}{\sqrt{V[X]V[Y]}} = \frac{0.006944444}{\sqrt{(0.07638889)(0.07638889)}} = 0.09090908$$

![Question_4](C:\Users\Sekhar\Documents\R Programs\Simulation\HW2\Q4.png)
*Answer:*

Let us read the given data to an R Vector

```{r}
x <- c(7.3,6.1, 3.8, 8.4, 6.9, 7.1, 5.3, 8.2, 4.9, 5.8)
mean(x)
var(x)


```

Therefore mean, $\overline{x} = 6.38$ and $s^2 = 2.161778$

To compute the 95% confidence interval for the population mean ($\mu$), we need to obtain the z-scores at the p-values 0.025 and 0.975 

```{r}
z_1 = qnorm(0.025)
z_2 = qnorm(0.975)

x_1 = z_1*sd(x)+mean(x)
x_2 = z_2*sd(x)+mean(x)

print(x_1)
print(x_2)

```

Therefore, the 95% confidence interval for $\mu$ is $[3.498268,9.261732]$

![Question_5](C:\Users\Sekhar\Documents\R Programs\Simulation\HW2\Q5.png)
*Answer:*

We can express $Pr(X > t+s | X >t)$ as

$$Pr(X > t+s | X>t) = \frac{Pr(X > t+s \cap x > t)}{Pr(X>t)}$$

Since $t$ and $s$ are always positive, we can say that $(s+t)$ is always greater than $t$. Hence $Pr(X > s+t \cap X >t)$ must be equal to $Pr(X > s+t)$

Therefore, 
$$Pr(X > t+s | X>t) = \frac{Pr(X > t+s)}{Pr(X>t)}$$

For the exponential distribution, the $c.d.f$ is

$$F(X \leq x) = 1 - e^\frac{-x}{\beta}$$
Therefore 
$$F(X \geq x) = e^\frac{-x}{\beta}$$

Where $\beta$ is the average of the exponential distribution.

Using exponential distribution $c.d.f$, we can write the above expression as:

$$Pr(X > t+s | X>t) = \frac{e^{\frac{-(t+s)}{\beta}}}{e^{\frac{-(t)}{\beta}}} = e^{\frac{-s}{\beta}} = Pr(X > s)$$

Hence, $Pr(X > t+s | X>t) = Pr(X > s)$, and the distribution is memoryless.

![Question_6](C:\Users\Sekhar\Documents\R Programs\Simulation\HW2\Q6.png)
*Answer:*

Given that $\lambda = 1$. Therefore the mean $\mu = \frac{1}{\lambda} = 1$ and standard deviation $\sigma =  \frac{1}{\lambda} = 1$

As per central limit theorem, if we draw random samples of size "n" from a distribution, then the mean of the samples will be approximately equal to the population mean, and the standard deviation of the sampling distribution will be $\sigma/\sqrt{n}$

In the problem, n = 100. Therefore standard deviation of the sampling distribution = $1/\sqrt{100} = 0.1$

$$Pr(100 \leq \sum_{i=1}^{100}X_i \leq 110) = Pr(1 \leq \sum_{i=1}^{100}\frac{X_i}{100} \leq 1.1)$$

(When dividing $100 \leq \sum_{i=1}^{100}X_i \leq 110$ by 100)

The z-scores of 1 and 1.1 (for a std. normal distribution with mean 1 and std. deviation of 0.1) are 0 and 1 respectively. The associated p-values for z-scores of 0 and 0.1 are 0.5 and 0.8413447 respectively. Therefore the $Pr(1 \leq \sum_{i=1}^{100}\frac{X_i}{100} \leq 1.1) = 0.8413447 - 0.5 = 0.3413447$


#Question 7 - 5.13 problem in DES book

##(a)
Given the $p.m.f$ as
$$p(x) =1/(n+1)$$ where x = {0,1,2,3...n}

$$E[X] = \sum_{x=0}^{x=n} x . (1/(n+1)) = \sum_{x=0}^{x=n} x /(n+1)$$

$$E[X] = \frac{1}{n+1} + \frac{2}{n+1} + \frac{3}{n+1} + ... + \frac{n}{n+1}$$
$$E[X] = \frac{1}{n+1}(1+2+3+...+n) = \frac{1}{n+1}(\frac{n(n+1)}{2}) = n/2$$
$$E[X] = n/2$$

$$V[X] = E[X^2] - (E[X])^2$$

$$E[X^2] = \sum_{x=0}^{x=n} x^2 . (1/(n+1)) = \sum_{x=0}^{x=n} x^2 /(n+1)$$

$$E[X^2] = \frac{1^2}{n+1} + \frac{2^2}{n+1} + \frac{3^2}{n+1} + ... + \frac{n^2}{n+1}$$
$$E[X^2] = \frac{1}{n+1}(1^2+2^2+3^3+...+n^2) = \frac{1}{n+1}(\frac{n(n+1)(2n+1)}{6}) = n(2n+1)/6$$


$$V[X] = E[X^2] - (E[X])^2 = \frac{n(2n+1)}{6} - (\frac{n}{2})^2 = (2n^2/6)+(n/6)-(n^2/4) = \frac{n^2+2n}{12}$$

##(b)

Given that $R_X = \{a,a+1,a+2,a+3,...,b\}$

If this is a discrete uniform distribution, then the $p.m.f$ is the reciprocal of the number of elements in the sample space, and hence for the given distribution, it can be written as:

$$P(X=x) = \frac{1}{b-a+1}$$

Let us find the E[X]:
$$E[X] = \sum_{i=a}^{b} i.\frac{1}{b-a+1}$$
$$E[X] = a.\frac{1}{b-a+1} + (a+1).\frac{1}{b-a+1} + (a+2).\frac{1}{b-a+1} ... + b.\frac{1}{b-a+1}$$
$$E[X] = \frac{1}{b-a+1} [a+(a+1)+(a+2)+(a+3)+...+b]$$


In the above expression, the sum of the consecutive numbers $[a+(a+1)+(a+2)+(a+3)+...+b]$ can be written as the difference between the sum of first $b$ natural numbers and the sum of first $(a-1)$ natural numbers.

$$[a+(a+1)+(a+2)+(a+3)+...+b] = \frac{b.(b+1)}{2} - \frac{a.(a-1)}{2} = \frac{b^2+b-a^2+a}{2} = \frac{(b+a)[b-a+1]}{2}$$

Hence, $$E[X] = \frac{1}{b-a+1} [a+(a+1)+(a+2)+(a+3)+...+b] = \frac{1}{b-a+1} . \frac{(b+a)[b-a+1]}{2} = \frac{b+a}{2}$$


$$V[X] = E[X^2] - (E[X])^2$$

$$E[X^2] = \sum_{i=a}^{b} i^2 \frac{1}{b-a+1}$$
$$E[X^2] = a^2 \frac{1}{b-a+1} + (a+1)^2 \frac{1}{b-a+1} +(a+2)^2 \frac{1}{b-a+1} + ... + b^2 \frac{1}{b-a+1}$$
$$E[X^2] = \frac{1}{b-a+1} [a^2 + (a+1)^2 + (a+2)^2 + ... + b^2]$$
$$\frac{1}{b-a+1} [a^2 + (a+1)^2 + (a+2)^2 + ... + b^2] = \frac{1}{b-a+1}[\frac{b.(b+1)(2b+1)}{6} - \frac{(a-1)(a)(2a-1)}{6}]$$
$$V[X] = E[X^2] - E[X] = \frac{1}{b-a+1}  [\frac{b.(b+1)(2b+1)}{6} - \frac{(a-1)(a)(2a-1)}{6}]- \frac{b^2+a^2+2ab}{4}$$

Upon simplifying, we will get:

$$V[X] = \frac{(b-a+1)^2- 1}{12}$$

##Alternate proof:
If we have $R_x = \{0,1,2,3...n\}$ as discrete uniform distribution sample space, then the expected value was computed as $n/2$. Now if we increase/decrease each element by a constant in the sample space by a constant $a$, then the E[X] will also get effected by the same value (increase/decrease by $a$). If we add $a$ to all the elements of $R_x = \{0,1,2,3...n\}$, we get $R_x = \{a,a+1,a+2...a+n\}$, which can be written as $R_x = \{a,a+1,a+2...b\}$, when you assume $a+n$ as $b$.

The number of elements will be $b-a+1$ (The number of elements in the distribution $R_x = \{0,1,2,3...n\}$ is $n+1$. Therefore $b-a+1 = n+1$, and $b-a=n$). 

The expected value will be (substitute $n=b-a$ in $n/2$:

$$E[X] = ((b-a+1) - 1)/2 + a$$ (since the average of n+1 elements $R_x = \{0,1,2,3...n\}$ is $n/2$, and also the resulting mean has to be transformed by $a$)
$$E[X] = ((b-a)/2 + a = (b+a)/2$$ 

The V[X] does not change, even though when we increment the distribution by a constant number $a$. So for the uniform discrete distribution (with $n+1$ elements) $R_x = \{0,1,2,3...n\}$, we know that the $V[X] = \frac{n^2+2n}{12}$. So when we increment each value of $R_x = \{0,1,2,3...n\}$ by $a$, the number of elements will be $b-a+1$. Hence, the V[X] will be
$$V[X] = \frac{(b-a)^2+2(b-a)}{12}$$
$$V[X] = \frac{(b-a)^2+2(b-a)}{12}$$
Adding and subtracting 1 to the numerator, will give:
$$V[X] = \frac{(b-a)^2+2(b-a) + 1 - 1}{12}$$
$$V[X] = \frac{(b-a+1)^2- 1}{12}$$


#Question 7 - 5.14 problem in DES book

Given the exponential distribution with $\lambda = 0.4$. Therefore mean = $1/\lambda = 1/0.4 = 2.5 years$

##(a)

The probability that the satillite lives more than 5 years is:

$$Pr(X > 5) = \int_{5}^{\infty} \frac{e^{\frac{-x}{2.5}}}{2.5} \mbox{ dx} = e^{-2} = 0.1353353$$



##(b)
The probability that the satillite dies between 3 and 6 years is:

$$Pr(3<X<6) = \int_{3}^{6} \frac{e^{\frac{-x}{2.5}}}{2.5} \mbox{ dx }$$

$$Pr(3<X<6) = e^{\frac{-3}{2.5}} - e^{\frac{-6}{2.5}} = 0.2104763$$


#Question 7 - 5.39 problem in DES book

##(a). 

The combined linkage will have normal distribution $N(150,0.25)$. This normal distribution's mean and variance are obtained by adding together the means and variances or the given 3 distributions respectively.

##(b)

The $P(Linkage > 150.2)$ can be found, by first identifying the z-score of 150.2 cm (for the mean 150 and variance of 0.25 normal distribution).

$$Z_{150.2} = \frac{150.2 - 150}{0.5} = 0.4$$

The area under the std. normal curve (for Z>0.4) is $1 - p(Z<0.4) = 1-0.6554217 = 0.3445783$

##(c)

$$Z_{149.83} = \frac{149.83 - 150}{0.5} = -0.34$$

$$Z_{150.21} = \frac{150.21 - 150}{0.5} = 0.42$$

p-value of -0.34 is $p(Z < -0.34)= 0.3669283$ and p-value of 0.42 is $P(Z<0.42) = 0.6627573$

Therefore the proportion of links which are between 149.83 cm and 150.2 cm is: $0.6627573 - 0.3669283 = 0.295829$



